adding a separate coercions module relating the various effects; revising the spec style of arrays; adding a few more utilities; commenting the .fstis

pulse/ulib/experimental/Steel.ST.Array.fst
@@ -17,6 +17,8 @@
 module Steel.ST.Array
 open FStar.Ghost
 open Steel.ST.Util
+open FStar.Seq
+open Steel.ST.Coercions
 module U32 = FStar.UInt32
 module A = Steel.Array
 module SEA = Steel.Effect.Atomic
@@ -33,12 +35,44 @@ let length (#t:_) (r:array t)
   : GTot nat
   = A.length r
 
+let repr (#t:_) (r:array t) = FStar.Seq.lseq t (length r)
+
 /// The main representation predicate
 let pts_to (#t:Type)
            (a:array t)
-           ([@@@smt_fallback]x:repr a)
+           ([@@@smt_fallback]x:seq t)
   : vprop
-  = A.varray_pts_to a x
+  = exists_ (fun (r:repr a) ->
+      pure (eq2 #(seq t) r x) `star`
+      A.varray_pts_to a r)
+
+let intro_pts_to #t #o (a:array t) (s:repr a) (s':seq t)
+  : STGhost unit o
+      (A.varray_pts_to a s)
+      (fun _ -> pts_to a s')
+      (requires s == s')
+      (ensures fun _ -> True)
+  = intro_pure (s == s');
+    intro_exists s (fun (s:repr a) -> pure (s == s') `star` A.varray_pts_to a s)
+
+let elim_pts_to #t #o (a:array t) (s:seq t)
+  : STGhost (erased (repr a)) o
+      (pts_to a s)
+      (fun s' -> A.varray_pts_to a s')
+      (requires True)
+      (ensures fun s' -> eq2 #(seq t) s' s)
+  = let s = elim_exists () in
+    elim_pure _;
+    s
+
+let pts_to_length #t #o (a:array t) (s:seq t)
+  : STGhost unit o
+      (pts_to a s)
+      (fun _ -> pts_to a s)
+      (requires True)
+      (ensures fun _ -> Seq.length s == length a)
+  = let s' = elim_pts_to a s in
+    intro_pts_to a s' s
 
 let alloc_pt (#t:Type)
              (x:t)
@@ -48,9 +82,7 @@ let alloc_pt (#t:Type)
            (fun r -> pts_to r (Seq.create (U32.v n) x))
   = let a = A.malloc x n in
     let s = A.intro_varray_pts_to a in
-    SEA.change_equal_slprop
-              (A.varray_pts_to _ _)
-              (pts_to _ _);
+    intro_pts_to a s (Seq.create (U32.v n) x);
     return a
 
 let alloc (#t:Type)
@@ -62,28 +94,29 @@ let alloc (#t:Type)
   = let x = coerce_steel (fun _ -> alloc_pt x n) in x
 
 let read_pt (#t:Type)
-            (a:array t)
-            (#s:erased (repr a))
-            (i:U32.t { U32.v i < length a })
+              (a:array t)
+              (#s:erased (seq t))
+               (i:U32.t { U32.v i < Seq.length s })
   : SE.Steel t
        (pts_to a s)
        (fun _ -> pts_to a s)
        (requires fun _ -> True)
        (ensures fun _ v _ ->
          v == Seq.index s (U32.v i))
-  = A.elim_varray_pts_to a s;
+  = let s' = elim_pts_to a s in
+    A.elim_varray_pts_to a s';
     let x = A.index a i in
     let _ = A.intro_varray_pts_to a in
     SEA.change_equal_slprop
               (A.varray_pts_to _ _)
-              (pts_to _ _);
+              (A.varray_pts_to _ _);
+    intro_pts_to a s' s;
     return x
-
 
 let read (#t:Type)
          (a:array t)
-         (#s:erased (repr a))
-         (i:U32.t { U32.v i < length a })
+         (#s:erased (seq t))
+         (i:U32.t { U32.v i < Seq.length s })
   : ST t
        (pts_to a s)
        (fun _ -> pts_to a s)
@@ -93,35 +126,33 @@ let read (#t:Type)
   = let x = coerce_steel (fun _ -> read_pt a i) in x
 
 let write_pt (#t:Type)
-          (a:array t)
-          (#s:erased (repr a))
-          (i:U32.t { U32.v i < length a })
-          (x:t)
+             (a:array t)
+             (#s:erased (seq t))
+             (i:U32.t { U32.v i < Seq.length s })
+             (x:t)
   : SE.SteelT unit
        (pts_to a s)
        (fun _ -> pts_to a (Seq.upd s (U32.v i) x))
-  = A.elim_varray_pts_to a s;
+  = let s' = elim_pts_to a s in
+    A.elim_varray_pts_to a s';
     A.upd a i x;
-    let _ = A.intro_varray_pts_to a in
-    SEA.change_equal_slprop
-              (A.varray_pts_to _ _)
-              (pts_to _ _);
+    let s'' = A.intro_varray_pts_to a in
+    intro_pts_to a _ _;
     return ()
 
 let write (#t:Type)
           (a:array t)
-          (#s:erased (repr a))
-          (i:U32.t { U32.v i < length a })
+          (#s:erased (seq t))
+          (i:U32.t { U32.v i < Seq.length s })
           (x:t)
   : STT unit
        (pts_to a s)
        (fun _ -> pts_to a (Seq.upd s (U32.v i) x))
   = coerce_steel (fun _ -> write_pt a i x); ()
 
-/// Frees array [r], as long as it initially was a valid array in memory
 let free_pt (#t:Type) (a:array t) (#s:erased (repr a))
   : SE.SteelT unit
-       (pts_to a s)
+       (A.varray_pts_to a s)
        (fun _ -> emp)
   = A.elim_varray_pts_to a s;
     A.free a;
@@ -131,35 +162,31 @@ let free (#t:Type) (a:array t)
   : STT unit
        (exists_ (pts_to a))
        (fun _ -> emp)
-  = let s = elim_exists () in
+  = let _ = elim_exists () in
+    let s = elim_pts_to a _ in
     coerce_steel (fun _ -> free_pt a #s)
-
 
 let memcpy_pt (#t:_)
               (a0 a1:array t)
-              (#s0:erased (repr a0))
-              (#s1:erased (repr a1))
+              (#s0 #s1:erased (seq t))
               (l:U32.t { U32.v l == length a0 /\ length a0 == length a1 } )
   : SE.SteelT unit
       (pts_to a0 s0 `star` pts_to a1 s1)
       (fun _ -> pts_to a0 s0  `star` pts_to a1 s0)
-  = A.elim_varray_pts_to a0 s0;
-    A.elim_varray_pts_to a1 s1;
+  = let _ = elim_pts_to a0 s0 in
+    let _ = elim_pts_to a1 s1 in
+    A.elim_varray_pts_to a0 _;
+    A.elim_varray_pts_to a1 _;
     A.memcpy a0 a1 l;
     let _ = A.intro_varray_pts_to a0 in
     let _ = A.intro_varray_pts_to a1 in
-    SEA.change_equal_slprop
-              (A.varray_pts_to a0 _)
-              (pts_to a0 _);
-    SEA.change_equal_slprop
-              (A.varray_pts_to a1 _)
-              (pts_to a1 _);
+    intro_pts_to a0 _ _;
+    intro_pts_to a1 _ _;
     return ()
 
 let memcpy (#t:_)
            (a0 a1:array t)
-           (#s0:erased (repr a0))
-           (#s1:erased (repr a1))
+           (#s0 #s1:erased (seq t))
            (l:U32.t { U32.v l == length a0 /\ length a0 == length a1 } )
   : STT unit
     (pts_to a0 s0 `star` pts_to a1 s1)
@@ -168,31 +195,27 @@ let memcpy (#t:_)
 
 let compare_pt (#t:eqtype)
                (a0 a1:array t)
-               (#s0:erased (repr a0))
-               (#s1:erased (repr a1))
+               (#s0 #s1:erased (seq t))
                (l:U32.t { U32.v l == length a0 /\ length a0 == length a1 } )
   : SE.Steel bool
     (pts_to a0 s0 `star` pts_to a1 s1)
     (fun _ -> pts_to a0 s0 `star` pts_to a1 s1)
     (requires fun _ -> True)
     (ensures fun _ b _ -> b <==> eq2 #(Seq.seq t) s0 s1)
-  = A.elim_varray_pts_to a0 s0;
-    A.elim_varray_pts_to a1 s1;
+  = let _ = elim_pts_to a0 _ in
+    let _ = elim_pts_to a1 _ in
+    A.elim_varray_pts_to a0 _;
+    A.elim_varray_pts_to a1 _;
     let b = A.compare a0 a1 l in
     let _ = A.intro_varray_pts_to a0 in
     let _ = A.intro_varray_pts_to a1 in
-    SEA.change_equal_slprop
-              (A.varray_pts_to a0 _)
-              (pts_to a0 _);
-    SEA.change_equal_slprop
-              (A.varray_pts_to a1 _)
-              (pts_to a1 _);
+    intro_pts_to a0 _ _;
+    intro_pts_to a1 _ _;
     return b
 
 let compare (#t:eqtype)
             (a0 a1:array t)
-            (#s0:erased (repr a0))
-            (#s1:erased (repr a1))
+            (#s0 #s1:erased (seq t))
             (l:U32.t { U32.v l == length a0 /\ length a0 == length a1 } )
   : ST bool
     (pts_to a0 s0 `star` pts_to a1 s1)
